src/lib/gen/NoModel.ml
@@ -74,35 +74,34 @@ let tableau_jumps a a0 a1 b =
             fix_F y)
   in fix_F (a,(a0,(a1,b)))
 
-(** val tableau : Assumptions.t -> CplSolver.t -> Mcnf0.t -> Solution.t **)
+(** val tableau : Mcnf0.t -> CplSolver.t -> Assumptions.t -> Solution.t **)
 
 let tableau a a0 b =
   let rec fix_F x =
-    let a1 = let pr1,_ = x in pr1 in
     let s0 = let pr1,_ = let _,pr2 = x in pr2 in pr1 in
+    let a1 = let _,pr2 = let _,pr2 = x in pr2 in pr2 in
     let tableau0 = fun a2 a3 b0 -> let y = a2,(a3,b0) in (fun _ -> fix_F y) in
     (match inspect (solve_with_assumptions s0 a1) with
      | Sat v ->
-       (match let _,pr2 = let _,pr2 = x in pr2 in pr2 with
+       (match let pr1,_ = x in pr1 with
         | [] -> Solution.Sat
         | t0 :: l ->
           (match inspect
                    (tableau_jumps v t0 l (fun a' ->
-                     tableau0 a' (make_with_clauses (first_cpls l)) l __)) with
+                     tableau0 l (cplsolver_mcnf l) a' __)) with
            | JumpSolution.Sat -> Solution.Sat
            | JumpSolution.Unsat (c, core) ->
              let conflict_set = conflict_set_of (t0 :: l) v c core in
              let s0' = CplSolver.add_conflict_set s0 conflict_set in
              let mc0' = add_conflict_set (t0 :: l) conflict_set in
-             tableau0 a1 s0' mc0' __))
+             tableau0 mc0' s0' a1 __))
      | Unsat core -> Solution.Unsat core)
   in fix_F (a,(a0,b))
 
 (** val solve_mcnf : Mcnf0.t -> Solution.t **)
 
 let solve_mcnf mc0 =
-  let cpls0 = first_cpls mc0 in
-  let s0 = make_with_clauses cpls0 in tableau [] s0 mc0
+  tableau mc0 (cplsolver_mcnf mc0) []
 
 (** val solve_fml : Fml.t -> Solution.t **)
 
