src/lib/gen/Spec.mli
@@ -50,7 +50,7 @@ val tableau_jumps :
   t -> Lclauses.t -> Mcnf0.t -> (Assumptions.t -> Solution.t) ->
   JumpSolution.t
 
-val tableau : Assumptions.t -> CplSolver.t -> Mcnf0.t -> Solution.t
+val tableau : Mcnf0.t -> CplSolver.t -> Assumptions.t -> Solution.t
 
 val solve_mcnf : Mcnf0.t -> Solution.t
 
